Progress on parameterization theorem.

src/Pyrosome/Compilers/Parameterizer.v
@@ -2,16 +2,37 @@ Set Implicit Arguments.
 Set Bullet Behavior "Strict Subproofs".
 
 Require Import String List.
+Require Import Bool.
 Import ListNotations.
 Open Scope string.
 Open Scope list.
-From Utils Require Import Utils Monad.
-From Pyrosome Require Import Theory.Core Compilers.CompilerDefs.
+From Utils Require Import Utils Infinite Monad.
+From Pyrosome Require Import Theory.Core Theory.Renaming Compilers.CompilerDefs.
 Import Core.Notations.
 
+(*TODO: move to Utils.v*)
+Definition unique_proofs P := forall (a b : P), a = b.
 
-(*TOOD: duplicated; move to Utils.v*)
-Definition inb {A} `{Eqb A} x := existsb (eqb x).
+Lemma is_true_unique : forall b, unique_proofs (Is_true b).
+Proof.
+  destruct b; intros a b;
+    destruct a; destruct b;
+    auto.
+Qed.
+
+Notation "'{B' x & c }" :=
+  (sigT (fun x => Is_true c))
+    (x binder, format "'[' '{B'  x  &  c } ']'").
+
+
+Lemma is_true_subset_eq {A} f (a b : {B x : A & f x})
+  : a = b <-> projT1 a = projT1 b.
+Proof.
+  destruct a; destruct b; simpl;
+    intuition try congruence; subst.
+  f_equal.
+  apply is_true_unique.
+Qed.
 
 (*TODO: move to Monad.v *)
 Definition named_list_Mmap {M V A B} `{Monad M} (f : A -> M B)
@@ -21,7 +42,9 @@ Definition named_list_Mmap {M V A B} `{Monad M} (f : A -> M B)
 Section WithVar.
   Context (V : Type)
           {V_Eqb : Eqb V}
-          {V_default : WithDefault V}.
+          {V_default : WithDefault V}
+  (*{V_inf : Infinite V}*).
+  
 
   Notation named_list := (@named_list V).
   Notation named_map := (@named_map V).
@@ -45,148 +68,342 @@ Section WithVar.
 
   Section WithParameter.
 
-    (*TODO: how to handle p_name freshness*)
+    (*TODO: how to handle p_name freshness?
+      idea: non-identity injective endofunction
+      - skip p_name in cod
+      - preserve lang vars (w/out proof they are in the lang)
+     *)
     Context (p_name : V)
-      (p_sort : sort).
+      (p_sort : sort)
+      (* assume a renaming where p_name isn't in the codomain *)
+      (f : V -> V)
+      (*TODO: make Injective a typeclass?*)
+      {f_inj : Injective f}
+      {p_name_fresh : forall x, f x <> p_name}.
+
+    Lemma p_name_freshb x : Is_true (negb (eqb (f x) p_name)).
+    Proof.
+      apply negb_prop_intro.
+      intro H.
+      apply p_name_fresh with (x:=x).
+      revert H; unfold Is_true; case_match;
+        basic_utils_crush.
+    Qed.
     
-    Section WithRules.    
-
-      Context (rules_to_parameterize : list V).
-
-        Fixpoint parameterize_term (e : term) : term :=
-          match e with
-          | var x => var x
-          | con n s =>
-              let s' := map parameterize_term s in
-              if inb n rules_to_parameterize
-              (*TODO: p_name freshness as fn of c.
-                  Question: should c already be parameterized?
-               *)
-              then con n (s'++[var p_name])
-              else con n s'
-          end.
-        
-        Definition parameterize_sort (e : sort) : sort :=
-          match e with
-          | scon n s =>
-              let s' := map parameterize_term s in
-              if inb n rules_to_parameterize
-                (*TODO: p_name freshness as fn of c.
-                  Question: should c already be parameterized?
-                 *)
-                then scon n (s'++[var p_name])
-                else scon n s'
-          end.
-
-        (*TODO: double-check when delta should be added.
-          E.G. sort w/ parametric arg must be parameterized
-          simple sort should not
-         *)
-        Definition parameterize_ctx (c : ctx) : ctx :=
-          (named_map parameterize_sort c)++[(p_name, p_sort)].
-
-        Definition parameterize_rule (r : rule) : rule :=
-          match r with
-          | sort_rule c args =>
-              sort_rule (parameterize_ctx c) args
-          | term_rule c args t =>
-              term_rule (parameterize_ctx c) args (parameterize_sort t)
-          | sort_eq_rule c t1 t2 =>
-              sort_eq_rule (parameterize_ctx c)
-                (parameterize_sort t1)
-                (parameterize_sort t2)
-          | term_eq_rule c e1 e2 t =>
-              term_eq_rule (parameterize_ctx c)
-                (parameterize_term e1)
-                (parameterize_term e2)
-                (parameterize_sort t)
-          end.
-
-        
-        Definition parameterize_ccase n c : compiler_case V :=
-          let ext_args :=
-            if inb n rules_to_parameterize
-            then fun a => a++[p_name]
-            else fun a => a
-          in
-          match c with
-          | sort_case args t =>
-              sort_case (ext_args args) (parameterize_sort t)
-          | term_case args e =>
-              term_case (ext_args args) (parameterize_term e)
-          end.
-
-        Fixpoint parameterize_compiler c : compiler V :=
-          match c with
-          | [] => []
-          | (n,cc)::c' =>
-              (n, parameterize_ccase n cc):: (parameterize_compiler c')
-          end.
-
-        Fixpoint should_parameterize_term (e : term) : bool :=
-          match e with
-          | var _ => false
-          | con n s =>
-              (inb n rules_to_parameterize)
-              || (existsb should_parameterize_term s)
-          end.
-
-        
-        Definition should_parameterize_sort t : bool :=
-          match t with
-          | scon n s =>
-              (inb n rules_to_parameterize)
-              || (existsb should_parameterize_term s)
-          end.
-
-        Definition should_parameterize_ctx : ctx -> _ :=
-          existsb (fun '(_,t) => should_parameterize_sort t).
-
-        Definition should_parameterize (r : rule) : bool :=
-          match r with
-          | sort_rule c args => (should_parameterize_ctx c)
-          | term_rule c args t =>
-              (should_parameterize_ctx c)
-              || (should_parameterize_sort t)
-          | sort_eq_rule c t1 t2 =>
-              (should_parameterize_ctx c)
-              || (should_parameterize_sort t1)
-              || (should_parameterize_sort t2)
-          | term_eq_rule c e1 e2 t =>
-              (should_parameterize_ctx c)
-              || (should_parameterize_term e1)
-              || (should_parameterize_term e2)
-              || (should_parameterize_sort t)
-          end.    
-        
-    End WithRules.
-
-    Fixpoint parameterize_lang' (l : lang) rules :=
-      match l with
-      | [] => ([], rules)
-      | (x,r)::l' =>
-          let (l'', rules') := parameterize_lang' l' rules in
-          if inb x rules'
-                 (*TODO: add to args in this case*)
-          then ((x,parameterize_rule rules r)::l'', rules')
-          else if should_parameterize rules' r
-               then ((x,parameterize_rule rules r)::l'', x::rules')
-               else ((x,r)::l'', rules')
+    (*TODO: move to Renaming?*)
+    Definition f' x : {B x & negb (eqb x p_name)} :=
+      existT _ (f x) (p_name_freshb x).
+    
+    Fixpoint parameterize_term (e : term) : term :=
+      match e with
+      | var x => var x
+      | con n s =>
+          let s' := map parameterize_term s in
+          con n (s'++[var p_name])
+      end.
+    
+    Definition parameterize_sort (e : sort) : sort :=
+      match e with
+      | scon n s =>
+          let s' := map parameterize_term s in
+          scon n (s'++[var p_name])
       end.
 
-    Definition parameterize_lang rules l : lang :=
-      fst (parameterize_lang' l rules).
+    (*TODO: double-check when delta should be added.
+          E.G. sort w/ parametric arg must be parameterized
+          simple sort should not
+     *)
+    Definition parameterize_ctx (c : ctx) : ctx :=
+      (named_map parameterize_sort c)++[(p_name, p_sort)].
 
+    Definition parameterize_sub s :=
+      (named_map parameterize_term s)++[(p_name, var p_name)].
+    
+    Definition parameterize_args s :=
+      (map parameterize_term s)++[var p_name].
+
+    Definition parameterize_rule (r : rule) : rule :=
+      match r with
+      | sort_rule c args =>
+          (*TODO: making p implicit in terms but not args is heuristic.
+                Give the user more control.
+           *)
+          sort_rule (parameterize_ctx c) (args++[p_name])
+      | term_rule c args t =>
+          term_rule (parameterize_ctx c) args (parameterize_sort t)
+      | sort_eq_rule c t1 t2 =>
+          sort_eq_rule (parameterize_ctx c)
+            (parameterize_sort t1)
+            (parameterize_sort t2)
+      | term_eq_rule c e1 e2 t =>
+          term_eq_rule (parameterize_ctx c)
+            (parameterize_term e1)
+            (parameterize_term e2)
+            (parameterize_sort t)
+      end.
+
+    
+    Definition parameterize_ccase (c : compiler_case V) : compiler_case V :=
+      match c with
+      | sort_case args t =>
+          sort_case (args++[p_name]) (parameterize_sort t)
+      | term_case args e =>
+          term_case (args++[p_name]) (parameterize_term e)
+      end.
+
+    Definition parameterize_compiler : _ -> compiler V :=
+      named_map parameterize_ccase.
+
+    Notation parameterize_lang := (named_map parameterize_rule).
+
+    
+    Lemma parameterize_subst_lookup s n e
+      : n <> p_name ->
+        parameterize_term (subst_lookup s n) =
+          subst_lookup (named_map parameterize_term s ++ [(p_name, e)]) n.
+    Proof.
+      intro.
+      induction s;
+        basic_goal_prep;
+        basic_term_crush.
+      {
+        apply eqb_neq in H.
+        rewrite H.
+        reflexivity.
+      }
+      {
+        case_match; auto.
+      }
+    Qed.
+
+    Lemma subst_lookup_p_name s
+      : fresh p_name s ->
+        subst_lookup (parameterize_sub s) p_name = var p_name.
+    Proof.
+      induction s;
+        basic_goal_prep;
+        basic_term_crush.
+      {
+        case_match;
+          basic_utils_crush.
+      }
+    Qed.
+
+    
+    Lemma p_name_not_in_map l
+      :  ~ In p_name (map f l).
+    Proof.
+      induction l;
+        basic_goal_prep;
+        basic_utils_crush.
+    Qed.        
+      
+    Lemma p_name_fresh_in_subst s
+      : fresh p_name (rename_subst f s).
+    Proof.
+      unfold rename_subst, fresh.
+      rewrite map_map; simpl.
+      rewrite <- map_map.
+      apply p_name_not_in_map.
+    Qed.
+
+    Lemma p_name_fresh_in_ctx s
+      : fresh p_name (rename_ctx f s).
+    Proof.
+      unfold rename_ctx, fresh.
+      rewrite map_map; simpl.
+      rewrite <- map_map.
+      apply p_name_not_in_map.
+    Qed.
+
+
+    
+    Lemma parameterize_term_subst e s
+      : parameterize_term (rename f e) [/rename_subst f s /]
+        = (parameterize_term (rename f e)) [/parameterize_sub (rename_subst f s) /].
+    Proof.
+      induction e;
+        basic_goal_prep;
+        basic_term_crush.
+      {
+        unfold parameterize_sub.
+        apply parameterize_subst_lookup; auto.
+        firstorder.
+      }
+      {
+        rewrite !map_app, !map_map;
+          simpl.
+        f_equal.
+        {
+          revert H.
+          induction l;
+            basic_goal_prep;
+            basic_term_crush.
+        }
+        {
+          f_equal.
+          rewrite subst_lookup_p_name; auto.
+          apply p_name_fresh_in_subst.
+        }
+      }
+    Qed.
+    
+    Lemma parameterize_args_subst e s
+      : parameterize_args (map (rename f) e) [/rename_subst f s /]
+        = (parameterize_args (map (rename f) e)) [/parameterize_sub (rename_subst f s) /].
+    Proof.
+      induction e;
+        basic_goal_prep;
+        basic_term_crush.
+      {
+        cbn; f_equal.
+        rewrite subst_lookup_p_name; auto.
+        apply p_name_fresh_in_subst.
+      }
+      {
+        cbn.
+        unfold parameterize_args in *.
+        fold_Substable.
+        f_equal; auto.
+        rewrite !parameterize_term_subst; eauto.
+      }
+    Qed.
+
+    Lemma parameterize_sort_subst e s
+      : parameterize_sort (rename_sort f e) [/rename_subst f s /]
+        = (parameterize_sort (rename_sort f e)) [/parameterize_sub (rename_subst f s) /].
+    Proof.
+      destruct e;
+        basic_goal_prep.
+      pose proof parameterize_args_subst as H';
+        unfold parameterize_args in H';
+        rewrite H'; eauto.
+    Qed.
+
+    (*TODO: move to Rule.v*)
+    Definition get_ctx (r : rule) :=
+      match r with
+      | sort_rule c _
+      | term_rule c _ _
+      | sort_eq_rule c _ _
+      | term_eq_rule c _ _ _ => c
+      end.
+
+    Lemma parameterization_monotonicity
+      l lp (l':= (parameterize_lang (rename_lang f l))++lp)
+      : all_fresh l' ->
+        (forall c t1 t2,
+            eq_sort l c t1 t2 ->
+            eq_sort l' (parameterize_ctx (rename_ctx f c))
+              (parameterize_sort (rename_sort f t1))
+              (parameterize_sort (rename_sort f t2)))
+        /\ (forall c t e1 e2,
+               eq_term l c t e1 e2 ->
+               eq_term l' (parameterize_ctx (rename_ctx f c))
+                 (parameterize_sort (rename_sort f t))
+                 (parameterize_term (rename f e1))
+                 (parameterize_term (rename f e2)))
+        /\ (forall c c' s1 s2,
+               eq_subst l c c' s1 s2 ->
+               eq_subst l' (parameterize_ctx (rename_ctx f c))
+                 (parameterize_ctx (rename_ctx f c'))
+                 (parameterize_sub (rename_subst f s1))
+                 (parameterize_sub (rename_subst f s2)))
+        /\ (forall c t,
+               wf_sort l c t ->
+               wf_sort l' (parameterize_ctx (rename_ctx f c))
+                 (parameterize_sort (rename_sort f t)))
+        /\ (forall c e t,
+               wf_term l c e t ->
+               wf_term l' (parameterize_ctx (rename_ctx f c))
+                 (parameterize_term (rename f e))
+                 (parameterize_sort (rename_sort f t)))
+        /\ (forall c s c',
+               wf_args l c s c' ->
+               wf_args l' (parameterize_ctx (rename_ctx f c))
+                 (parameterize_args (map (rename f) s))
+                 (parameterize_ctx (rename_ctx f c)))
+        /\ (forall c,
+               wf_ctx l c ->
+               wf_ctx l' (parameterize_ctx (rename_ctx f c))).
+Proof using.
+  intros all_fresh.
+  apply judge_ind; basic_goal_prep.
+  all: try solve [constructor; eauto].
+  all: erewrite ?rename_sort_distr_subst, ?rename_distr_subst by assumption.
+  all: rewrite ?parameterize_term_subst, ?parameterize_sort_subst.
+  {
+    subst l'.
+    eapply eq_sort_by.
+    eapply in_or_app; left.
+    unfold parameterize_lang, rename_lang.
+    rewrite map_map; simpl.
+    eapply in_map in H; exact H.
+  }
+  1:basic_core_crush.
+  1:basic_core_crush.
+  1:solve [basic_core_crush].
+  
+  {
+    subst l'.
+    eapply eq_term_by.
+    eapply in_or_app; left.
+    unfold parameterize_lang, rename_lang.
+    rewrite map_map; simpl.
+    eapply in_map in H; exact H.
+  }  
+  1:solve [basic_core_crush].
+  1:solve [basic_core_crush].
+  {
+    cbn.
+    repeat constructor.
+    unfold parameterize_ctx.
+    basic_utils_crush.
+    right.
+    simpl.
+    left.
+    f_equal.
+    admit (*TODO: find lemma*).
+  }
+  {
+    cbn.
+    constructor; basic_core_crush.
+    TODO: need hypothesis to be in terms of V = V - p_name
+  1:solve [basic_core_crush].
+  1:solve [basic_core_crush].
+  1:solve [basic_core_crush].
+  1:solve [basic_core_crush].
+  1:solve [basic_core_crush].
+  1:solve [basic_core_crush].
+  {
+    basic_core_crush.
+    TODO: why are s1, s2 not renamed?
+    rewrite <- !rename_sort_distr_subst.
+     all: rewrite <- ?parameterize_term_subst, <- ?parameterize_sort_subst.
+ 
+    Idea: rename via V -> V' renaming, using a subset type
+
+    all: rewrite ?parameterize_term_subst, ?parameterize_sort_subst.
+    TODO: how to rename? generalize mutual inductive to include list of reserved names?
+      - relies on V being infinite
+    eapply eq_sort_subst; cycle 1; eauto. }
+  {
+    TODO: what to do about ctxs in eq_sort_subst? alpha-rename? cut elim?
+    alpha:                                                          
+    pair of lemmas for renaming a ctx
+  }
+  constructor. eauto].
+    eauto.
+    rewrite parameterize_sort_subst; eauto.
+      TODO: commute w/ subst
+Qed.
+    
     End WithParameter.
 
 End WithVar.
 
 Require Import Pyrosome.Lang.SimpleVSubst.
 
-Compute (parameterize_lang' "D" {{s #"ty_env"}}
+Compute (parameterize_lang "D" {{s #"ty_env"}}
            value_subst
-           ["env"; "ty"; "sub"; "exp"; "val"]
         ).
-(*
-TODO: what's the benefit (ignoring inference) over just parameterizing everything?
-*)
