src/Pyrosome/Theory/Renaming.v
@@ -1,0 +1,244 @@
+Set Implicit Arguments.
+Set Bullet Behavior "Strict Subproofs".
+
+Require Import String List.
+Import ListNotations.
+Open Scope string.
+Open Scope list.
+From Utils Require Import Utils Monad.
+From Pyrosome Require Import Theory.Core.
+
+
+
+#[local] Notation eq_subst l :=
+  (eq_subst (Model:= core_model l)).
+#[local] Notation eq_args l :=
+  (eq_args (Model:= core_model l)).
+#[local] Notation wf_subst l :=
+  (wf_subst (Model:= core_model l)).
+#[local] Notation wf_args l :=
+  (wf_args (Model:= core_model l)).
+#[local] Notation wf_ctx l :=
+  (wf_ctx (Model:= core_model l)).
+
+
+(*TODO: check if this is defined somewhere.
+    If not, move it to Utils.v
+ *)
+Definition Injective {A B : Type} (f : A -> B) := forall a a', f a = f a' -> a = a'.
+
+Section Injective.
+  Context (A B : Type)
+    `{Eqb A}
+    `{Eqb B}
+    (f : A -> B)
+    (f_inj : Injective f).
+
+  
+  Lemma injective_in a l
+    : In (f a) (map f l) ->
+      In a l.
+  Proof.
+    induction l; basic_goal_prep; basic_utils_crush.
+  Qed.
+
+  #[local] Hint Resolve injective_in : utils.
+  
+
+  Fixpoint rename e :=
+    match e with
+    | var n => var (f n)
+    | con n l => con (f n) (map rename l)
+    end.
+
+  
+  Definition rename_subst : subst A -> _:=
+    map (fun p => (f (fst p), rename (snd p))).
+  
+  Definition rename_sort t :=
+    match t with
+    | scon n l => scon (f n) (map rename l)
+    end.
+
+  Definition rename_ctx : ctx A -> _:=
+    map (fun p => (f (fst p), rename_sort (snd p))).
+
+  Definition rename_rule r :=
+    match r with
+    | sort_rule c args => sort_rule (rename_ctx c) (map f args)
+    | term_rule c args t => term_rule (rename_ctx c) (map f args) (rename_sort t)
+    | sort_eq_rule c t t' => sort_eq_rule (rename_ctx c) (rename_sort t) (rename_sort t')
+    | term_eq_rule c e e' t =>
+        term_eq_rule (rename_ctx c) (rename e) (rename e') (rename_sort t)
+    end.
+  
+  Definition rename_lang : lang A -> _ :=
+    map (fun p => (f (fst p), rename_rule (snd p))).
+
+  Lemma rename_lookup s n
+    : rename (subst_lookup s n) = subst_lookup (rename_subst s) (f n).
+  Proof.
+    induction s; basic_goal_prep; repeat case_match; basic_term_crush.
+    symmetry in HeqH1.
+    basic_utils_crush.
+  Qed.
+
+  (*TODO: make this export?*)
+  #[local] Hint Rewrite rename_lookup : term.
+  
+  (*TODO: make this export & move to Utils?*)
+  #[local] Hint Rewrite map_map : utils.
+  
+  Lemma rename_distr_subst e s
+    : rename e[/s/] = (rename e) [/rename_subst s/].
+  Proof.
+    induction e; basic_goal_prep; basic_term_crush.
+    revert H1.
+    induction l; basic_goal_prep; basic_term_crush.
+  Qed.
+  
+  #[local] Hint Rewrite rename_distr_subst : term.
+
+  
+  Lemma rename_args_distr_subst e s
+    : map rename e[/s/] = (map rename e) [/rename_subst s/].
+  Proof.
+    induction e; basic_goal_prep; fold_Substable; basic_term_crush.
+  Qed.
+  
+  #[local] Hint Rewrite rename_args_distr_subst : term.
+
+  
+  Lemma rename_sort_distr_subst e s
+    : rename_sort e[/s/] = (rename_sort e) [/rename_subst s/].
+  Proof.
+    destruct e; basic_goal_prep; basic_term_crush.
+  Qed.
+  
+  #[local] Hint Rewrite rename_sort_distr_subst : term.
+
+  
+  Lemma rename_subst_distr_with_names_from c' s
+    : rename_subst (with_names_from c' s)
+      = with_names_from (rename_ctx c') (map rename s).
+  Proof.
+    revert s;
+      induction c';
+      destruct s;
+      basic_goal_prep; fold_Substable; basic_term_crush.
+  Qed.
+  
+  #[local] Hint Rewrite rename_subst_distr_with_names_from : term.
+  
+
+  Local Lemma rename_mono l
+    : (forall c t1 t2,
+          eq_sort l c t1 t2 ->
+          eq_sort (rename_lang l) (rename_ctx c) (rename_sort t1) (rename_sort t2))
+      /\ (forall c t e1 e2,
+             eq_term l c t e1 e2 ->
+             eq_term (rename_lang l) (rename_ctx c) (rename_sort t) (rename e1) (rename e2))
+      /\ (forall c c' s1 s2,
+             eq_subst l c c' s1 s2 ->
+             eq_subst (rename_lang l) (rename_ctx c) (rename_ctx c')
+               (rename_subst s1) (rename_subst s2))
+      /\ (forall c t,
+             wf_sort l c t ->
+             wf_sort (rename_lang l) (rename_ctx c) (rename_sort t))
+      /\ (forall c e t,
+             wf_term l c e t ->
+             wf_term (rename_lang l) (rename_ctx c) (rename e) (rename_sort t))
+      /\ (forall c s c',
+             wf_args l c s c' ->
+             wf_args (rename_lang l) (rename_ctx c) (map rename s) (rename_ctx c'))
+      /\ (forall c,
+             wf_ctx l c ->
+             wf_ctx (rename_lang l) (rename_ctx c)).
+  Proof using f_inj.
+    apply judge_ind; basic_goal_prep.
+    all:
+      let l := lazymatch goal with l : lang _ |- _ => l end in
+      try lazymatch goal with
+          H : In _ l |- _ => 
+            eapply in_map in H
+        end.
+    {
+      eapply eq_sort_by.
+      exact H1.
+    }
+    all: basic_core_crush.
+    {
+      eapply eq_term_by.
+      exact H1.
+    }
+    {
+      eapply wf_sort_by; eauto.
+      exact H1.
+    }
+    {
+      eapply wf_term_by; eauto.
+      exact H1.
+    }
+    {
+      eapply wf_term_var; eauto.
+      eapply in_map in H1.
+      exact H1.
+    }
+    {
+      intro.
+      apply H1.
+      eapply injective_in.
+      revert H6.
+      unfold rename_ctx.
+      rewrite !map_map; simpl; auto.
+    }
+  Qed.
+  
+End Injective.
+
+Section Inverse.
+  
+  Context (A B : Type)
+    `{Eqb A}
+    `{Eqb B}
+    (f : A -> B)
+    (g : B -> A)
+    (f_g_inverse : forall a, g (f a) = a).
+
+  #[local] Lemma f_inj : Injective f.
+  Proof.      
+    intros a a' Heq.
+    congruence.
+  Qed.
+
+  Lemma rename_inverse e
+    : rename g (rename f e) = e.
+  Proof.
+    induction e; basic_goal_prep; repeat case_match; basic_term_crush.
+    revert H1.
+    induction l; basic_goal_prep; repeat case_match; basic_term_crush.
+  Qed.
+
+  #[local] Hint Rewrite rename_inverse : term.
+  
+  Lemma rename_inverse_args s
+    : map (rename g) (map (rename f) s) = s.
+  Proof.
+    induction s; basic_goal_prep; repeat case_match; basic_term_crush.
+  Qed.
+
+  #[local] Hint Rewrite rename_inverse_args : term.
+  
+  Lemma rename_inverse_sort e
+    : rename_sort g (rename_sort f e) = e.
+  Proof.
+    induction e; basic_goal_prep; repeat case_match; basic_term_crush.
+  Qed.
+
+  #[local] Hint Rewrite rename_inverse_sort : term.
+
+End Inverse.
+  
+
+    (*TODO: rules about renaming inverses*)
+
