src/Utils/Infinite.v
@@ -1,0 +1,56 @@
+Set Implicit Arguments.
+Set Bullet Behavior "Strict Subproofs".
+
+Require Import List String Ascii.
+From Utils Require Import Utils.
+
+(* A class for using the infiniteness of types,
+   designed to be convenient to use constructively.
+   Note: this class is still for proof purposes
+   and instances may have poor performance
+ *)
+Class Infinite (V : Type) := {
+    gensym : list V -> V
+  }.
+
+Class Infinite_ok (V : Type) `{Infinite V} := {
+    gensym_ok : forall l, ~ In (gensym l) l
+  }.
+
+Arguments Infinite_ok V%type_scope {H}.
+ 
+#[export] Instance string_infinite : Infinite string :=
+  {
+    gensym l :=
+      let len := S (list_max (map length l)) in
+      string_of_list_ascii (repeat "!"%char len)
+  }.
+
+(*TODO: move to Utils.v*)
+Lemma string_of_list_ascii_length l
+  : length (string_of_list_ascii l) = List.length l.
+Proof.
+  induction l;
+    basic_goal_prep;
+    basic_utils_crush.
+Qed.
+
+#[export] Instance string_infinite_ok : Infinite_ok string.
+Proof.
+  constructor; unfold gensym, string_infinite.
+  intro l.
+  set (string_of_list_ascii _) as s.
+  intro HIn.
+  assert ((list_max (map length l))< length s).
+  {
+    subst s.
+    rewrite string_of_list_ascii_length, repeat_length.
+    auto.
+  }
+  assert (map length l <> nil) by (destruct l; simpl; basic_utils_crush).
+  epose proof (list_max_lt _ H0).
+  apply H1 in H.
+  assert (In (length s) (map length l)) by eauto using in_map.
+  eapply Forall_forall in H; eauto.
+  eapply PeanoNat.Nat.lt_irrefl; eauto.
+Qed.
